soundness: generated F* models

ristretto255/proofs/fstar/extraction/Ristretto255.Bundle.fst
@@ -10,7 +10,243 @@ let _ =
   let open Subtle in
   ()
 
+/// A compressed Ristretto255 point.
+/// This represents the canonical encoding of a Ristretto255 group element.
+type t_CompressedRistretto =
+  | CompressedRistretto : t_Array u8 (mk_usize 32) -> t_CompressedRistretto
+
+let impl_13: Core_models.Clone.t_Clone t_CompressedRistretto =
+  { f_clone = (fun x -> x); f_clone_pre = (fun _ -> True); f_clone_post = (fun _ _ -> True) }
+
+[@@ FStar.Tactics.Typeclasses.tcinstance]
+assume
+val impl_12': Core_models.Marker.t_Copy t_CompressedRistretto
+
+unfold
+let impl_12 = impl_12'
+
+[@@ FStar.Tactics.Typeclasses.tcinstance]
+assume
+val impl_14': Core_models.Fmt.t_Debug t_CompressedRistretto
+
+unfold
+let impl_14 = impl_14'
+
+[@@ FStar.Tactics.Typeclasses.tcinstance]
+assume
+val impl_16': Core_models.Hash.t_Hash t_CompressedRistretto
+
+unfold
+let impl_16 = impl_16'
+
+[@@ FStar.Tactics.Typeclasses.tcinstance]
+let impl_17: Core_models.Cmp.t_PartialEq t_CompressedRistretto t_CompressedRistretto =
+  {
+    f_eq_pre = (fun (self: t_CompressedRistretto) (other: t_CompressedRistretto) -> true);
+    f_eq_post
+    =
+    (fun (self: t_CompressedRistretto) (other: t_CompressedRistretto) (out: bool) -> true);
+    f_eq
+    =
+    fun (self: t_CompressedRistretto) (other: t_CompressedRistretto) ->
+      Core_models.Convert.f_into #Subtle.t_Choice
+        #bool
+        #FStar.Tactics.Typeclasses.solve
+        (Subtle.f_ct_eq #(t_Slice u8)
+            #FStar.Tactics.Typeclasses.solve
+            (self._0 <: t_Slice u8)
+            (other._0 <: t_Slice u8)
+          <:
+          Subtle.t_Choice)
+  }
+
+[@@ FStar.Tactics.Typeclasses.tcinstance]
+assume
+val impl_15': Core_models.Cmp.t_Eq t_CompressedRistretto
+
+unfold
+let impl_15 = impl_15'
+
+/// Copy the bytes of this `CompressedRistretto`.
+let impl_19__to_bytes (self: t_CompressedRistretto) : t_Array u8 (mk_usize 32) = self._0
+
+/// View this `CompressedRistretto` as an array of bytes.
+let impl_19__as_bytes (self: t_CompressedRistretto) : t_Array u8 (mk_usize 32) = self._0
+
+[@@ FStar.Tactics.Typeclasses.tcinstance]
+let impl_18: Subtle.t_ConstantTimeEq t_CompressedRistretto =
+  {
+    f_ct_eq_pre = (fun (self: t_CompressedRistretto) (other: t_CompressedRistretto) -> true);
+    f_ct_eq_post
+    =
+    (fun (self: t_CompressedRistretto) (other: t_CompressedRistretto) (out: Subtle.t_Choice) -> true
+    );
+    f_ct_eq
+    =
+    fun (self: t_CompressedRistretto) (other: t_CompressedRistretto) ->
+      Subtle.f_ct_eq #(t_Slice u8)
+        #FStar.Tactics.Typeclasses.solve
+        (impl_19__as_bytes self <: t_Slice u8)
+        (impl_19__as_bytes other <: t_Slice u8)
+  }
+
+/// Construct a `CompressedRistretto` from a slice of bytes.
+/// # Errors
+/// Returns [`TryFromSliceError`] if the input `bytes` slice does not have
+/// a length of 32.
+let impl_19__from_slice (bytes: t_Slice u8)
+    : Prims.Pure
+      (Core_models.Result.t_Result t_CompressedRistretto Core_models.Array.t_TryFromSliceError)
+      (requires True)
+      (fun _ -> Prims.l_True) =
+  Core_models.Result.impl__map #(t_Array u8 (mk_usize 32))
+    #Core_models.Array.t_TryFromSliceError
+    #t_CompressedRistretto
+    (Core_models.Convert.f_try_into #(t_Slice u8)
+        #(t_Array u8 (mk_usize 32))
+        #FStar.Tactics.Typeclasses.solve
+        bytes
+      <:
+      Core_models.Result.t_Result (t_Array u8 (mk_usize 32)) Core_models.Array.t_TryFromSliceError)
+    CompressedRistretto
+
+[@@ FStar.Tactics.Typeclasses.tcinstance]
+let impl: Ristretto255.Traits.t_Identity t_CompressedRistretto =
+  {
+    f_identity_pre = (fun (_: Prims.unit) -> true);
+    f_identity_post = (fun (_: Prims.unit) (out: t_CompressedRistretto) -> true);
+    f_identity
+    =
+    fun (_: Prims.unit) ->
+      CompressedRistretto (Rust_primitives.Hax.repeat (mk_u8 0) (mk_usize 32))
+      <:
+      t_CompressedRistretto
+  }
+
+[@@ FStar.Tactics.Typeclasses.tcinstance]
+let impl_1: Core_models.Default.t_Default t_CompressedRistretto =
+  {
+    f_default_pre = (fun (_: Prims.unit) -> true);
+    f_default_post = (fun (_: Prims.unit) (out: t_CompressedRistretto) -> true);
+    f_default
+    =
+    fun (_: Prims.unit) ->
+      Ristretto255.Traits.f_identity #t_CompressedRistretto #FStar.Tactics.Typeclasses.solve ()
+  }
+
+[@@ FStar.Tactics.Typeclasses.tcinstance]
+let impl_20: Core_models.Convert.t_TryFrom t_CompressedRistretto (t_Slice u8) =
+  {
+    f_Error = Core_models.Array.t_TryFromSliceError;
+    f_try_from_pre = (fun (slice: t_Slice u8) -> true);
+    f_try_from_post
+    =
+    (fun
+        (slice: t_Slice u8)
+        (out:
+          Core_models.Result.t_Result t_CompressedRistretto Core_models.Array.t_TryFromSliceError)
+        ->
+        true);
+    f_try_from = fun (slice: t_Slice u8) -> impl_19__from_slice slice
+  }
+
+[@@ FStar.Tactics.Typeclasses.tcinstance]
+let impl_4: Core_models.Convert.t_From (t_Array u8 (mk_usize 32)) t_CompressedRistretto =
+  {
+    f_from_pre = (fun (c: t_CompressedRistretto) -> true);
+    f_from_post = (fun (c: t_CompressedRistretto) (out: t_Array u8 (mk_usize 32)) -> true);
+    f_from = fun (c: t_CompressedRistretto) -> c._0
+  }
+
+/// The compressed Ristretto255 basepoint (i.e. 1 * generator).
+let v_RISTRETTO_BASEPOINT_COMPRESSED: t_CompressedRistretto =
+  CompressedRistretto
+  (let list =
+      [
+        mk_u8 226; mk_u8 242; mk_u8 174; mk_u8 10; mk_u8 106; mk_u8 188; mk_u8 78; mk_u8 113;
+        mk_u8 168; mk_u8 132; mk_u8 169; mk_u8 97; mk_u8 197; mk_u8 0; mk_u8 81; mk_u8 95; mk_u8 88;
+        mk_u8 227; mk_u8 11; mk_u8 106; mk_u8 165; mk_u8 130; mk_u8 221; mk_u8 141; mk_u8 182;
+        mk_u8 166; mk_u8 89; mk_u8 69; mk_u8 224; mk_u8 141; mk_u8 45; mk_u8 118
+      ]
+    in
+    FStar.Pervasives.assert_norm (Prims.eq2 (List.Tot.length list) 32);
+    Rust_primitives.Hax.array_of_list 32 list)
+  <:
+  t_CompressedRistretto
+
 type t_FieldElement = | FieldElement : t_Array u64 (mk_usize 5) -> t_FieldElement
+
+/// An `EdwardsPoint` represents a point on the Edwards form of Curve25519
+/// in extended coordinates \\((X:Y:Z:T)\\) with \\(x = X/Z\\), \\(y = Y/Z\\),
+/// \\(xy = T/Z\\).
+type t_EdwardsPoint = {
+  f_X:t_FieldElement;
+  f_Y:t_FieldElement;
+  f_Z:t_FieldElement;
+  f_T:t_FieldElement
+}
+
+/// A `RistrettoPoint` is an element in the Ristretto255 group.
+type t_RistrettoPoint = | RistrettoPoint : t_EdwardsPoint -> t_RistrettoPoint
+
+let impl_22: Core_models.Clone.t_Clone t_RistrettoPoint =
+  { f_clone = (fun x -> x); f_clone_pre = (fun _ -> True); f_clone_post = (fun _ _ -> True) }
+
+[@@ FStar.Tactics.Typeclasses.tcinstance]
+assume
+val impl_21': Core_models.Marker.t_Copy t_RistrettoPoint
+
+unfold
+let impl_21 = impl_21'
+
+let impl_8__from__backend: Core_models.Clone.t_Clone t_EdwardsPoint =
+  { f_clone = (fun x -> x); f_clone_pre = (fun _ -> True); f_clone_post = (fun _ _ -> True) }
+
+[@@ FStar.Tactics.Typeclasses.tcinstance]
+assume
+val impl_7__from__backend': Core_models.Marker.t_Copy t_EdwardsPoint
+
+unfold
+let impl_7__from__backend = impl_7__from__backend'
+
+/// A `CompletedPoint` is a point \\(((X:Z), (Y:T))\\) on the
+/// \\(\mathbb P^1 \times \mathbb P^1\\) model of the curve.
+/// A point (x,y) in the affine model corresponds to \\(((x:1),(y:1))\\).
+type t_CompletedPoint = {
+  f_X:t_FieldElement;
+  f_Y:t_FieldElement;
+  f_Z:t_FieldElement;
+  f_T:t_FieldElement
+}
+
+let impl_10__from__backend: Core_models.Clone.t_Clone t_CompletedPoint =
+  { f_clone = (fun x -> x); f_clone_pre = (fun _ -> True); f_clone_post = (fun _ _ -> True) }
+
+[@@ FStar.Tactics.Typeclasses.tcinstance]
+assume
+val impl_9__from__backend': Core_models.Marker.t_Copy t_CompletedPoint
+
+unfold
+let impl_9__from__backend = impl_9__from__backend'
+
+/// A pre-computed point on the \\( \mathbb P\^3 \\) model for the
+/// curve, represented as \\((Y+X, Y-X, Z, 2dXY)\\) in "Niels coordinates".
+type t_ProjectiveNielsPoint = {
+  f_Y_plus_X:t_FieldElement;
+  f_Y_minus_X:t_FieldElement;
+  f_Z:t_FieldElement;
+  f_T2d:t_FieldElement
+}
+
+let impl_12__from__backend: Core_models.Clone.t_Clone t_ProjectiveNielsPoint =
+  { f_clone = (fun x -> x); f_clone_pre = (fun _ -> True); f_clone_post = (fun _ _ -> True) }
+
+[@@ FStar.Tactics.Typeclasses.tcinstance]
+assume
+val impl_11__from__backend': Core_models.Marker.t_Copy t_ProjectiveNielsPoint
+
+unfold
+let impl_11__from__backend = impl_11__from__backend'
 
 /// Edwards `d` value, equal to `-121665/121666 mod p`.
 let v_EDWARDS_D: t_FieldElement =
@@ -46,29 +282,131 @@ let v_SQRT_M1: t_FieldElement =
   <:
   t_FieldElement
 
-let impl_1: Core_models.Clone.t_Clone t_FieldElement =
+/// `= 1/sqrt(a-d)`, where `a = -1 (mod p)`, `d` are the Edwards curve parameters.
+let v_INVSQRT_A_MINUS_D: t_FieldElement =
+  FieldElement
+  (let list =
+      [
+        mk_u64 278908739862762;
+        mk_u64 821645201101625;
+        mk_u64 8113234426968;
+        mk_u64 1777959178193151;
+        mk_u64 2118520810568447
+      ]
+    in
+    FStar.Pervasives.assert_norm (Prims.eq2 (List.Tot.length list) 5);
+    Rust_primitives.Hax.array_of_list 5 list)
+  <:
+  t_FieldElement
+
+/// One minus edwards `d` value squared, equal to `(1 - (-121665/121666) mod p) pow 2`
+let v_ONE_MINUS_EDWARDS_D_SQUARED: t_FieldElement =
+  FieldElement
+  (let list =
+      [
+        mk_u64 1136626929484150;
+        mk_u64 1998550399581263;
+        mk_u64 496427632559748;
+        mk_u64 118527312129759;
+        mk_u64 45110755273534
+      ]
+    in
+    FStar.Pervasives.assert_norm (Prims.eq2 (List.Tot.length list) 5);
+    Rust_primitives.Hax.array_of_list 5 list)
+  <:
+  t_FieldElement
+
+/// Edwards `d` value minus one squared, equal to `(((-121665/121666) mod p) - 1) pow 2`
+let v_EDWARDS_D_MINUS_ONE_SQUARED: t_FieldElement =
+  FieldElement
+  (let list =
+      [
+        mk_u64 1507062230895904;
+        mk_u64 1572317787530805;
+        mk_u64 683053064812840;
+        mk_u64 317374165784489;
+        mk_u64 1572899562415810
+      ]
+    in
+    FStar.Pervasives.assert_norm (Prims.eq2 (List.Tot.length list) 5);
+    Rust_primitives.Hax.array_of_list 5 list)
+  <:
+  t_FieldElement
+
+/// `= sqrt(a*d - 1)`, where `a = -1 (mod p)`, `d` are the Edwards curve parameters.
+let v_SQRT_AD_MINUS_ONE: t_FieldElement =
+  FieldElement
+  (let list =
+      [
+        mk_u64 2241493124984347;
+        mk_u64 425987919032274;
+        mk_u64 2207028919301688;
+        mk_u64 1220490630685848;
+        mk_u64 974799131293748
+      ]
+    in
+    FStar.Pervasives.assert_norm (Prims.eq2 (List.Tot.length list) 5);
+    Rust_primitives.Hax.array_of_list 5 list)
+  <:
+  t_FieldElement
+
+/// The value of minus one, equal to `-&FieldElement::ONE`
+let v_MINUS_ONE: t_FieldElement =
+  FieldElement
+  (let list =
+      [
+        mk_u64 2251799813685228;
+        mk_u64 2251799813685247;
+        mk_u64 2251799813685247;
+        mk_u64 2251799813685247;
+        mk_u64 2251799813685247
+      ]
+    in
+    FStar.Pervasives.assert_norm (Prims.eq2 (List.Tot.length list) 5);
+    Rust_primitives.Hax.array_of_list 5 list)
+  <:
+  t_FieldElement
+
+/// Edwards `2*d` value, equal to `2*(-121665/121666) mod p`.
+let v_EDWARDS_D2: t_FieldElement =
+  FieldElement
+  (let list =
+      [
+        mk_u64 1859910466990425;
+        mk_u64 932731440258426;
+        mk_u64 1072319116312658;
+        mk_u64 1815898335770999;
+        mk_u64 633789495995903
+      ]
+    in
+    FStar.Pervasives.assert_norm (Prims.eq2 (List.Tot.length list) 5);
+    Rust_primitives.Hax.array_of_list 5 list)
+  <:
+  t_FieldElement
+
+let impl_1__from__field: Core_models.Clone.t_Clone t_FieldElement =
   { f_clone = (fun x -> x); f_clone_pre = (fun _ -> True); f_clone_post = (fun _ _ -> True) }
 
 [@@ FStar.Tactics.Typeclasses.tcinstance]
 assume
-val impl_2': Core_models.Marker.t_Copy t_FieldElement
+val impl_2__from__field': Core_models.Marker.t_Copy t_FieldElement
 
 unfold
-let impl_2 = impl_2'
+let impl_2__from__field = impl_2__from__field'
 
 [@@ FStar.Tactics.Typeclasses.tcinstance]
 assume
-val impl_3': Core_models.Fmt.t_Debug t_FieldElement
+val impl_3__from__field': Core_models.Fmt.t_Debug t_FieldElement
 
 unfold
-let impl_3 = impl_3'
+let impl_3__from__field = impl_3__from__field'
 
 [@@ FStar.Tactics.Typeclasses.tcinstance]
 assume
-val impl_4': Core_models.Marker.t_StructuralPartialEq t_FieldElement
+val impl_4__from__field': Core_models.Marker.t_StructuralPartialEq t_FieldElement
 
 unfold
-let impl_4 = impl_4'
+let impl_4__from__field = impl_4__from__field'
 
 [@@ FStar.Tactics.Typeclasses.tcinstance]
 assume
@@ -79,13 +417,13 @@ let impl_5 = impl_5'
 
 [@@ FStar.Tactics.Typeclasses.tcinstance]
 assume
-val impl_6': Core_models.Cmp.t_Eq t_FieldElement
+val impl_6__from__field': Core_models.Cmp.t_Eq t_FieldElement
 
 unfold
-let impl_6 = impl_6'
+let impl_6__from__field = impl_6__from__field'
 
 [@@ FStar.Tactics.Typeclasses.tcinstance]
-let impl: Ristretto255.Traits.t_Identity t_FieldElement =
+let impl__from__field: Ristretto255.Traits.t_Identity t_FieldElement =
   {
     f_identity_pre = (fun (_: Prims.unit) -> true);
     f_identity_post = (fun (_: Prims.unit) (out: t_FieldElement) -> true);
@@ -96,7 +434,7 @@ let impl: Ristretto255.Traits.t_Identity t_FieldElement =
   }
 
 [@@ FStar.Tactics.Typeclasses.tcinstance]
-let impl_8: Core_models.Ops.Arith.t_Add t_FieldElement t_FieldElement =
+let impl_8__from__field: Core_models.Ops.Arith.t_Add t_FieldElement t_FieldElement =
   {
     f_Output = t_FieldElement;
     f_add_pre = (fun (self: t_FieldElement) (rhs: t_FieldElement) -> true);
@@ -112,7 +450,7 @@ let impl_8: Core_models.Ops.Arith.t_Add t_FieldElement t_FieldElement =
   }
 
 [@@ FStar.Tactics.Typeclasses.tcinstance]
-let impl_9: Core_models.Ops.Arith.t_Sub t_FieldElement t_FieldElement =
+let impl_9__from__field: Core_models.Ops.Arith.t_Sub t_FieldElement t_FieldElement =
   {
     f_Output = t_FieldElement;
     f_sub_pre = (fun (self: t_FieldElement) (rhs: t_FieldElement) -> true);
@@ -128,7 +466,7 @@ let impl_9: Core_models.Ops.Arith.t_Sub t_FieldElement t_FieldElement =
   }
 
 [@@ FStar.Tactics.Typeclasses.tcinstance]
-let impl_10: Core_models.Ops.Arith.t_Mul t_FieldElement u64 =
+let impl_10__from__field: Core_models.Ops.Arith.t_Mul t_FieldElement u64 =
   {
     f_Output = t_FieldElement;
     f_mul_pre = (fun (self: t_FieldElement) (rhs: u64) -> true);
@@ -144,7 +482,7 @@ let impl_10: Core_models.Ops.Arith.t_Mul t_FieldElement u64 =
   }
 
 [@@ FStar.Tactics.Typeclasses.tcinstance]
-let impl_11: Core_models.Ops.Arith.t_Mul t_FieldElement t_FieldElement =
+let impl_11__from__field: Core_models.Ops.Arith.t_Mul t_FieldElement t_FieldElement =
   {
     f_Output = t_FieldElement;
     f_mul_pre = (fun (self: t_FieldElement) (rhs: t_FieldElement) -> true);
@@ -172,9 +510,72 @@ let impl_11: Core_models.Ops.Arith.t_Mul t_FieldElement t_FieldElement =
 /// Equivalent to `(1u64 << 51) - 1`
 let v_LOW_51_BIT_MASK: u64 = mk_u64 2251799813685247
 
+let impl_12__ZERO: t_FieldElement =
+  FieldElement
+  (let list = [mk_u64 0; mk_u64 0; mk_u64 0; mk_u64 0; mk_u64 0] in
+    FStar.Pervasives.assert_norm (Prims.eq2 (List.Tot.length list) 5);
+    Rust_primitives.Hax.array_of_list 5 list)
+  <:
+  t_FieldElement
+
 let impl_12__ONE: t_FieldElement =
   FieldElement
   (let list = [mk_u64 1; mk_u64 0; mk_u64 0; mk_u64 0; mk_u64 0] in
+    FStar.Pervasives.assert_norm (Prims.eq2 (List.Tot.length list) 5);
+    Rust_primitives.Hax.array_of_list 5 list)
+  <:
+  t_FieldElement
+
+[@@ FStar.Tactics.Typeclasses.tcinstance]
+let impl__from__backend: Ristretto255.Traits.t_Identity t_EdwardsPoint =
+  {
+    f_identity_pre = (fun (_: Prims.unit) -> true);
+    f_identity_post = (fun (_: Prims.unit) (out: t_EdwardsPoint) -> true);
+    f_identity
+    =
+    fun (_: Prims.unit) ->
+      { f_X = impl_12__ZERO; f_Y = impl_12__ONE; f_Z = impl_12__ONE; f_T = impl_12__ZERO }
+      <:
+      t_EdwardsPoint
+  }
+
+[@@ FStar.Tactics.Typeclasses.tcinstance]
+let impl_6: Ristretto255.Traits.t_Identity t_RistrettoPoint =
+  {
+    f_identity_pre = (fun (_: Prims.unit) -> true);
+    f_identity_post = (fun (_: Prims.unit) (out: t_RistrettoPoint) -> true);
+    f_identity
+    =
+    fun (_: Prims.unit) ->
+      RistrettoPoint
+      (Ristretto255.Traits.f_identity #t_EdwardsPoint #FStar.Tactics.Typeclasses.solve ())
+      <:
+      t_RistrettoPoint
+  }
+
+[@@ FStar.Tactics.Typeclasses.tcinstance]
+let impl_7: Core_models.Default.t_Default t_RistrettoPoint =
+  {
+    f_default_pre = (fun (_: Prims.unit) -> true);
+    f_default_post = (fun (_: Prims.unit) (out: t_RistrettoPoint) -> true);
+    f_default
+    =
+    fun (_: Prims.unit) ->
+      Ristretto255.Traits.f_identity #t_RistrettoPoint #FStar.Tactics.Typeclasses.solve ()
+  }
+
+/// The scalar \\\\( -1 \\\\).
+let impl_12__MINUS_ONE: t_FieldElement =
+  FieldElement
+  (let list =
+      [
+        mk_u64 2251799813685228;
+        mk_u64 2251799813685247;
+        mk_u64 2251799813685247;
+        mk_u64 2251799813685247;
+        mk_u64 2251799813685247
+      ]
+    in
     FStar.Pervasives.assert_norm (Prims.eq2 (List.Tot.length list) 5);
     Rust_primitives.Hax.array_of_list 5 list)
   <:
@@ -189,7 +590,7 @@ unfold
 let impl_12__to_bytes = impl_12__to_bytes'
 
 [@@ FStar.Tactics.Typeclasses.tcinstance]
-let impl_7: Subtle.t_ConstantTimeEq t_FieldElement =
+let impl_7__from__field: Subtle.t_ConstantTimeEq t_FieldElement =
   {
     f_ct_eq_pre = (fun (self: t_FieldElement) (other: t_FieldElement) -> true);
     f_ct_eq_post
@@ -310,6 +711,13 @@ let impl_12__conditional_assign (self other: t_FieldElement) (choice: Subtle.t_C
   in
   self
 
+/// Raise this field element to the power (p-5)/8 = 2^252 - 3.
+assume
+val impl_12__pow_p58': self: t_FieldElement -> t_FieldElement
+
+unfold
+let impl_12__pow_p58 = impl_12__pow_p58'
+
 let impl_12__load8_at (input: t_Array u8 (mk_usize 32)) (i: usize)
     : Prims.Pure u64 (requires Rust_primitives.Integers.v i + 7 < 32) (fun _ -> Prims.l_True) =
   (((((((cast (input.[ i ] <: u8) <: u64) |.
@@ -354,8 +762,22 @@ let impl_12__from_bytes (bytes: t_Array u8 (mk_usize 32)) : t_FieldElement =
   <:
   t_FieldElement
 
+let step_1_ (repr: t_CompressedRistretto) : (Subtle.t_Choice & Subtle.t_Choice & t_FieldElement) =
+  let s:t_FieldElement = impl_12__from_bytes (impl_19__as_bytes repr <: t_Array u8 (mk_usize 32)) in
+  let s_bytes_check:t_Array u8 (mk_usize 32) = impl_12__to_bytes s in
+  let s_encoding_is_canonical:Subtle.t_Choice =
+    Subtle.f_ct_eq #(t_Slice u8)
+      #FStar.Tactics.Typeclasses.solve
+      (s_bytes_check.[ Core_models.Ops.Range.RangeFull <: Core_models.Ops.Range.t_RangeFull ]
+        <:
+        t_Slice u8)
+      (impl_19__as_bytes repr <: t_Slice u8)
+  in
+  let s_is_negative:Subtle.t_Choice = impl_12__is_negative s in
+  s_encoding_is_canonical, s_is_negative, s <: (Subtle.t_Choice & Subtle.t_Choice & t_FieldElement)
+
 [@@ FStar.Tactics.Typeclasses.tcinstance]
-let impl_13: Core_models.Ops.Arith.t_Add t_FieldElement t_FieldElement =
+let impl_13__from__field: Core_models.Ops.Arith.t_Add t_FieldElement t_FieldElement =
   {
     f_Output = t_FieldElement;
     f_add_pre = (fun (self: t_FieldElement) (rhs: t_FieldElement) -> true);
@@ -371,7 +793,7 @@ let impl_13: Core_models.Ops.Arith.t_Add t_FieldElement t_FieldElement =
   }
 
 [@@ FStar.Tactics.Typeclasses.tcinstance]
-let impl_14: Core_models.Ops.Arith.t_Sub t_FieldElement t_FieldElement =
+let impl_14__from__field: Core_models.Ops.Arith.t_Sub t_FieldElement t_FieldElement =
   {
     f_Output = t_FieldElement;
     f_sub_pre = (fun (self: t_FieldElement) (rhs: t_FieldElement) -> true);
@@ -387,7 +809,7 @@ let impl_14: Core_models.Ops.Arith.t_Sub t_FieldElement t_FieldElement =
   }
 
 [@@ FStar.Tactics.Typeclasses.tcinstance]
-let impl_15: Core_models.Ops.Arith.t_Mul t_FieldElement t_FieldElement =
+let impl_15__from__field: Core_models.Ops.Arith.t_Mul t_FieldElement t_FieldElement =
   {
     f_Output = t_FieldElement;
     f_mul_pre = (fun (self: t_FieldElement) (rhs: t_FieldElement) -> true);
@@ -402,46 +824,388 @@ let impl_15: Core_models.Ops.Arith.t_Mul t_FieldElement t_FieldElement =
         rhs
   }
 
-/// Raise this field element to the power (p-5)/8 = 2^252 - 3.
-let impl_12__pow_p58 (self: t_FieldElement) : t_FieldElement =
-  let acc:t_FieldElement = impl_12__ONE in
-  let acc:t_FieldElement =
-    Core_models.Iter.Traits.Iterator.f_fold (Core_models.Iter.Traits.Collect.f_into_iter #(Core_models.Iter.Adapters.Rev.t_Rev
-            (Core_models.Ops.Range.t_Range i32))
+[@@ FStar.Tactics.Typeclasses.tcinstance]
+let impl_9: Subtle.t_ConstantTimeEq t_RistrettoPoint =
+  {
+    f_ct_eq_pre = (fun (self: t_RistrettoPoint) (other: t_RistrettoPoint) -> true);
+    f_ct_eq_post
+    =
+    (fun (self: t_RistrettoPoint) (other: t_RistrettoPoint) (out: Subtle.t_Choice) -> true);
+    f_ct_eq
+    =
+    fun (self: t_RistrettoPoint) (other: t_RistrettoPoint) ->
+      let v_X1Y2:t_FieldElement =
+        Core_models.Ops.Arith.f_mul #t_FieldElement
+          #t_FieldElement
           #FStar.Tactics.Typeclasses.solve
-          (Core_models.Iter.Traits.Iterator.f_rev #(Core_models.Ops.Range.t_Range i32)
-              #FStar.Tactics.Typeclasses.solve
-              ({
-                  Core_models.Ops.Range.f_start = mk_i32 0;
-                  Core_models.Ops.Range.f_end = mk_i32 252
-                }
-                <:
-                Core_models.Ops.Range.t_Range i32)
-            <:
-            Core_models.Iter.Adapters.Rev.t_Rev (Core_models.Ops.Range.t_Range i32))
-        <:
-        Core_models.Iter.Adapters.Rev.t_Rev (Core_models.Ops.Range.t_Range i32))
-      acc
-      (fun acc i ->
-          let acc:t_FieldElement = acc in
-          let i:i32 = i in
-          let acc:t_FieldElement = impl_12__square acc in
-          if i <>. mk_i32 1
-          then
-            let acc:t_FieldElement =
-              Core_models.Ops.Arith.f_mul #t_FieldElement
-                #t_FieldElement
-                #FStar.Tactics.Typeclasses.solve
-                acc
-                self
-            in
-            acc
-          else acc)
-  in
-  acc
+          self._0.f_X
+          other._0.f_Y
+      in
+      let v_Y1X2:t_FieldElement =
+        Core_models.Ops.Arith.f_mul #t_FieldElement
+          #t_FieldElement
+          #FStar.Tactics.Typeclasses.solve
+          self._0.f_Y
+          other._0.f_X
+      in
+      let v_X1X2:t_FieldElement =
+        Core_models.Ops.Arith.f_mul #t_FieldElement
+          #t_FieldElement
+          #FStar.Tactics.Typeclasses.solve
+          self._0.f_X
+          other._0.f_X
+      in
+      let v_Y1Y2:t_FieldElement =
+        Core_models.Ops.Arith.f_mul #t_FieldElement
+          #t_FieldElement
+          #FStar.Tactics.Typeclasses.solve
+          self._0.f_Y
+          other._0.f_Y
+      in
+      Core_models.Ops.Bit.f_bitor #Subtle.t_Choice
+        #Subtle.t_Choice
+        #FStar.Tactics.Typeclasses.solve
+        (Subtle.f_ct_eq #t_FieldElement #FStar.Tactics.Typeclasses.solve v_X1Y2 v_Y1X2
+          <:
+          Subtle.t_Choice)
+        (Subtle.f_ct_eq #t_FieldElement #FStar.Tactics.Typeclasses.solve v_X1X2 v_Y1Y2
+          <:
+          Subtle.t_Choice)
+  }
 
 [@@ FStar.Tactics.Typeclasses.tcinstance]
-let impl_16: Core_models.Ops.Arith.t_Neg t_FieldElement =
+let impl_8: Core_models.Cmp.t_PartialEq t_RistrettoPoint t_RistrettoPoint =
+  {
+    f_eq_pre = (fun (self: t_RistrettoPoint) (other: t_RistrettoPoint) -> true);
+    f_eq_post = (fun (self: t_RistrettoPoint) (other: t_RistrettoPoint) (out: bool) -> true);
+    f_eq
+    =
+    fun (self: t_RistrettoPoint) (other: t_RistrettoPoint) ->
+      Core_models.Convert.f_into #Subtle.t_Choice
+        #bool
+        #FStar.Tactics.Typeclasses.solve
+        (Subtle.f_ct_eq #t_RistrettoPoint #FStar.Tactics.Typeclasses.solve self other
+          <:
+          Subtle.t_Choice)
+  }
+
+[@@ FStar.Tactics.Typeclasses.tcinstance]
+assume
+val impl_23': Core_models.Cmp.t_Eq t_RistrettoPoint
+
+unfold
+let impl_23 = impl_23'
+
+[@@ FStar.Tactics.Typeclasses.tcinstance]
+let impl_1__from__backend: Subtle.t_ConstantTimeEq t_EdwardsPoint =
+  {
+    f_ct_eq_pre = (fun (self: t_EdwardsPoint) (other: t_EdwardsPoint) -> true);
+    f_ct_eq_post
+    =
+    (fun (self: t_EdwardsPoint) (other: t_EdwardsPoint) (out: Subtle.t_Choice) -> true);
+    f_ct_eq
+    =
+    fun (self: t_EdwardsPoint) (other: t_EdwardsPoint) ->
+      Core_models.Ops.Bit.f_bitand #Subtle.t_Choice
+        #Subtle.t_Choice
+        #FStar.Tactics.Typeclasses.solve
+        (Subtle.f_ct_eq #t_FieldElement
+            #FStar.Tactics.Typeclasses.solve
+            (Core_models.Ops.Arith.f_mul #t_FieldElement
+                #t_FieldElement
+                #FStar.Tactics.Typeclasses.solve
+                self.f_X
+                other.f_Z
+              <:
+              t_FieldElement)
+            (Core_models.Ops.Arith.f_mul #t_FieldElement
+                #t_FieldElement
+                #FStar.Tactics.Typeclasses.solve
+                other.f_X
+                self.f_Z
+              <:
+              t_FieldElement)
+          <:
+          Subtle.t_Choice)
+        (Subtle.f_ct_eq #t_FieldElement
+            #FStar.Tactics.Typeclasses.solve
+            (Core_models.Ops.Arith.f_mul #t_FieldElement
+                #t_FieldElement
+                #FStar.Tactics.Typeclasses.solve
+                self.f_Y
+                other.f_Z
+              <:
+              t_FieldElement)
+            (Core_models.Ops.Arith.f_mul #t_FieldElement
+                #t_FieldElement
+                #FStar.Tactics.Typeclasses.solve
+                other.f_Y
+                self.f_Z
+              <:
+              t_FieldElement)
+          <:
+          Subtle.t_Choice)
+  }
+
+[@@ FStar.Tactics.Typeclasses.tcinstance]
+let impl_2: Core_models.Cmp.t_PartialEq t_EdwardsPoint t_EdwardsPoint =
+  {
+    f_eq_pre = (fun (self: t_EdwardsPoint) (other: t_EdwardsPoint) -> true);
+    f_eq_post = (fun (self: t_EdwardsPoint) (other: t_EdwardsPoint) (out: bool) -> true);
+    f_eq
+    =
+    fun (self: t_EdwardsPoint) (other: t_EdwardsPoint) ->
+      Core_models.Convert.f_into #Subtle.t_Choice
+        #bool
+        #FStar.Tactics.Typeclasses.solve
+        (Subtle.f_ct_eq #t_EdwardsPoint #FStar.Tactics.Typeclasses.solve self other
+          <:
+          Subtle.t_Choice)
+  }
+
+[@@ FStar.Tactics.Typeclasses.tcinstance]
+let impl_3: Core_models.Cmp.t_Eq t_EdwardsPoint = { _super_i0 = FStar.Tactics.Typeclasses.solve }
+
+/// Convert to a ProjectiveNielsPoint
+let impl_4__as_projective_niels (self: t_EdwardsPoint) : t_ProjectiveNielsPoint =
+  {
+    f_Y_plus_X
+    =
+    Core_models.Ops.Arith.f_add #t_FieldElement
+      #t_FieldElement
+      #FStar.Tactics.Typeclasses.solve
+      self.f_Y
+      self.f_X;
+    f_Y_minus_X
+    =
+    Core_models.Ops.Arith.f_sub #t_FieldElement
+      #t_FieldElement
+      #FStar.Tactics.Typeclasses.solve
+      self.f_Y
+      self.f_X;
+    f_Z = self.f_Z;
+    f_T2d
+    =
+    Core_models.Ops.Arith.f_mul #t_FieldElement
+      #t_FieldElement
+      #FStar.Tactics.Typeclasses.solve
+      self.f_T
+      v_EDWARDS_D2
+  }
+  <:
+  t_ProjectiveNielsPoint
+
+/// Convert this point from the \\( \mathbb P\^1 \times \mathbb P\^1
+/// \\) model to the \\( \mathbb P\^3 \\) model.
+/// This costs \\(4 \mathrm M \\).
+let impl_4__as_extended (self: t_EdwardsPoint) : t_EdwardsPoint =
+  {
+    f_X
+    =
+    Core_models.Ops.Arith.f_mul #t_FieldElement
+      #t_FieldElement
+      #FStar.Tactics.Typeclasses.solve
+      self.f_X
+      self.f_T;
+    f_Y
+    =
+    Core_models.Ops.Arith.f_mul #t_FieldElement
+      #t_FieldElement
+      #FStar.Tactics.Typeclasses.solve
+      self.f_Y
+      self.f_Z;
+    f_Z
+    =
+    Core_models.Ops.Arith.f_mul #t_FieldElement
+      #t_FieldElement
+      #FStar.Tactics.Typeclasses.solve
+      self.f_Z
+      self.f_T;
+    f_T
+    =
+    Core_models.Ops.Arith.f_mul #t_FieldElement
+      #t_FieldElement
+      #FStar.Tactics.Typeclasses.solve
+      self.f_X
+      self.f_Y
+  }
+  <:
+  t_EdwardsPoint
+
+/// Convert from the \\(\mathbb P^1 \times \mathbb P^1\\) model to
+/// the \\(\mathbb P^3\\) (extended) model.
+/// Cost: \\(4 \mathrm M\\).
+let impl_5__as_extended (self: t_CompletedPoint) : t_EdwardsPoint =
+  {
+    f_X
+    =
+    Core_models.Ops.Arith.f_mul #t_FieldElement
+      #t_FieldElement
+      #FStar.Tactics.Typeclasses.solve
+      self.f_X
+      self.f_T;
+    f_Y
+    =
+    Core_models.Ops.Arith.f_mul #t_FieldElement
+      #t_FieldElement
+      #FStar.Tactics.Typeclasses.solve
+      self.f_Y
+      self.f_Z;
+    f_Z
+    =
+    Core_models.Ops.Arith.f_mul #t_FieldElement
+      #t_FieldElement
+      #FStar.Tactics.Typeclasses.solve
+      self.f_Z
+      self.f_T;
+    f_T
+    =
+    Core_models.Ops.Arith.f_mul #t_FieldElement
+      #t_FieldElement
+      #FStar.Tactics.Typeclasses.solve
+      self.f_X
+      self.f_Y
+  }
+  <:
+  t_EdwardsPoint
+
+[@@ FStar.Tactics.Typeclasses.tcinstance]
+let impl_6__from__backend: Core_models.Ops.Arith.t_Add t_EdwardsPoint t_ProjectiveNielsPoint =
+  {
+    f_Output = t_CompletedPoint;
+    f_add_pre = (fun (self: t_EdwardsPoint) (other: t_ProjectiveNielsPoint) -> true);
+    f_add_post
+    =
+    (fun (self: t_EdwardsPoint) (other: t_ProjectiveNielsPoint) (out: t_CompletedPoint) -> true);
+    f_add
+    =
+    fun (self: t_EdwardsPoint) (other: t_ProjectiveNielsPoint) ->
+      let v_Y_plus_X:t_FieldElement =
+        Core_models.Ops.Arith.f_add #t_FieldElement
+          #t_FieldElement
+          #FStar.Tactics.Typeclasses.solve
+          self.f_Y
+          self.f_X
+      in
+      let v_Y_minus_X:t_FieldElement =
+        Core_models.Ops.Arith.f_sub #t_FieldElement
+          #t_FieldElement
+          #FStar.Tactics.Typeclasses.solve
+          self.f_Y
+          self.f_X
+      in
+      let v_PP:t_FieldElement =
+        Core_models.Ops.Arith.f_mul #t_FieldElement
+          #t_FieldElement
+          #FStar.Tactics.Typeclasses.solve
+          v_Y_plus_X
+          other.f_Y_plus_X
+      in
+      let v_MM:t_FieldElement =
+        Core_models.Ops.Arith.f_mul #t_FieldElement
+          #t_FieldElement
+          #FStar.Tactics.Typeclasses.solve
+          v_Y_minus_X
+          other.f_Y_minus_X
+      in
+      let v_TT2d:t_FieldElement =
+        Core_models.Ops.Arith.f_mul #t_FieldElement
+          #t_FieldElement
+          #FStar.Tactics.Typeclasses.solve
+          self.f_T
+          other.f_T2d
+      in
+      let v_ZZ:t_FieldElement =
+        Core_models.Ops.Arith.f_mul #t_FieldElement
+          #t_FieldElement
+          #FStar.Tactics.Typeclasses.solve
+          self.f_Z
+          other.f_Z
+      in
+      let v_ZZ2:t_FieldElement =
+        Core_models.Ops.Arith.f_add #t_FieldElement
+          #t_FieldElement
+          #FStar.Tactics.Typeclasses.solve
+          v_ZZ
+          v_ZZ
+      in
+      {
+        f_X
+        =
+        Core_models.Ops.Arith.f_sub #t_FieldElement
+          #t_FieldElement
+          #FStar.Tactics.Typeclasses.solve
+          v_PP
+          v_MM;
+        f_Y
+        =
+        Core_models.Ops.Arith.f_add #t_FieldElement
+          #t_FieldElement
+          #FStar.Tactics.Typeclasses.solve
+          v_PP
+          v_MM;
+        f_Z
+        =
+        Core_models.Ops.Arith.f_add #t_FieldElement
+          #t_FieldElement
+          #FStar.Tactics.Typeclasses.solve
+          v_ZZ2
+          v_TT2d;
+        f_T
+        =
+        Core_models.Ops.Arith.f_sub #t_FieldElement
+          #t_FieldElement
+          #FStar.Tactics.Typeclasses.solve
+          v_ZZ2
+          v_TT2d
+      }
+      <:
+      t_CompletedPoint
+  }
+
+[@@ FStar.Tactics.Typeclasses.tcinstance]
+let impl_10: Core_models.Ops.Arith.t_Add t_RistrettoPoint t_RistrettoPoint =
+  {
+    f_Output = t_RistrettoPoint;
+    f_add_pre = (fun (self: t_RistrettoPoint) (other: t_RistrettoPoint) -> true);
+    f_add_post
+    =
+    (fun (self: t_RistrettoPoint) (other: t_RistrettoPoint) (out: t_RistrettoPoint) -> true);
+    f_add
+    =
+    fun (self: t_RistrettoPoint) (other: t_RistrettoPoint) ->
+      RistrettoPoint
+      (impl_5__as_extended (Core_models.Ops.Arith.f_add #t_EdwardsPoint
+              #t_ProjectiveNielsPoint
+              #FStar.Tactics.Typeclasses.solve
+              self._0
+              (impl_4__as_projective_niels other._0 <: t_ProjectiveNielsPoint)
+            <:
+            t_CompletedPoint))
+      <:
+      t_RistrettoPoint
+  }
+
+[@@ FStar.Tactics.Typeclasses.tcinstance]
+let impl_11: Core_models.Ops.Arith.t_Add t_RistrettoPoint t_RistrettoPoint =
+  {
+    f_Output = t_RistrettoPoint;
+    f_add_pre = (fun (self: t_RistrettoPoint) (other: t_RistrettoPoint) -> true);
+    f_add_post
+    =
+    (fun (self: t_RistrettoPoint) (other: t_RistrettoPoint) (out: t_RistrettoPoint) -> true);
+    f_add
+    =
+    fun (self: t_RistrettoPoint) (other: t_RistrettoPoint) ->
+      Core_models.Ops.Arith.f_add #t_RistrettoPoint
+        #t_RistrettoPoint
+        #FStar.Tactics.Typeclasses.solve
+        self
+        other
+  }
+
+[@@ FStar.Tactics.Typeclasses.tcinstance]
+let impl_16__from__field: Core_models.Ops.Arith.t_Neg t_FieldElement =
   {
     f_Output = t_FieldElement;
     f_neg_pre = (fun (self: t_FieldElement) -> true);
@@ -459,7 +1223,7 @@ let impl_16: Core_models.Ops.Arith.t_Neg t_FieldElement =
   }
 
 [@@ FStar.Tactics.Typeclasses.tcinstance]
-let impl_17: Core_models.Ops.Arith.t_Neg t_FieldElement =
+let impl_17__from__field: Core_models.Ops.Arith.t_Neg t_FieldElement =
   {
     f_Output = t_FieldElement;
     f_neg_pre = (fun (self: t_FieldElement) -> true);
@@ -576,6 +1340,199 @@ let impl_12__sqrt_ratio_i (u v: t_FieldElement) : (Subtle.t_Choice & t_FieldElem
   in
   was_nonzero_square, r <: (Subtle.t_Choice & t_FieldElement)
 
+/// Computes the Ristretto Elligator map for the given field element. This is the second half of
+/// the [`MAP`](https://www.rfc-editor.org/rfc/rfc9496.html#section-4.3.4-4) function defined in
+/// the Ristretto spec.
+/// # Note
+/// This method is not public because it's just used for hashing
+/// to a point -- proper elligator support is deferred for now.
+let impl_3__elligator_ristretto_flavor (r_0_: t_FieldElement) : t_RistrettoPoint =
+  let i:t_FieldElement = v_SQRT_M1 in
+  let d:t_FieldElement = v_EDWARDS_D in
+  let one_minus_d_sq:t_FieldElement = v_ONE_MINUS_EDWARDS_D_SQUARED in
+  let d_minus_one_sq:t_FieldElement = v_EDWARDS_D_MINUS_ONE_SQUARED in
+  let c:t_FieldElement = v_MINUS_ONE in
+  let one:t_FieldElement = impl_12__ONE in
+  let r:t_FieldElement =
+    Core_models.Ops.Arith.f_mul #t_FieldElement
+      #t_FieldElement
+      #FStar.Tactics.Typeclasses.solve
+      i
+      (impl_12__square r_0_ <: t_FieldElement)
+  in
+  let v_N_s:t_FieldElement =
+    Core_models.Ops.Arith.f_mul #t_FieldElement
+      #t_FieldElement
+      #FStar.Tactics.Typeclasses.solve
+      (Core_models.Ops.Arith.f_add #t_FieldElement
+          #t_FieldElement
+          #FStar.Tactics.Typeclasses.solve
+          r
+          one
+        <:
+        t_FieldElement)
+      one_minus_d_sq
+  in
+  let v_D:t_FieldElement =
+    Core_models.Ops.Arith.f_mul #t_FieldElement
+      #t_FieldElement
+      #FStar.Tactics.Typeclasses.solve
+      (Core_models.Ops.Arith.f_sub #t_FieldElement
+          #t_FieldElement
+          #FStar.Tactics.Typeclasses.solve
+          c
+          (Core_models.Ops.Arith.f_mul #t_FieldElement
+              #t_FieldElement
+              #FStar.Tactics.Typeclasses.solve
+              d
+              r
+            <:
+            t_FieldElement)
+        <:
+        t_FieldElement)
+      (Core_models.Ops.Arith.f_add #t_FieldElement
+          #t_FieldElement
+          #FStar.Tactics.Typeclasses.solve
+          r
+          d
+        <:
+        t_FieldElement)
+  in
+  let (v_Ns_D_is_sq: Subtle.t_Choice), (s: t_FieldElement) = impl_12__sqrt_ratio_i v_N_s v_D in
+  let s_prime:t_FieldElement =
+    Core_models.Ops.Arith.f_mul #t_FieldElement
+      #t_FieldElement
+      #FStar.Tactics.Typeclasses.solve
+      s
+      r_0_
+  in
+  let s_prime_is_pos:Subtle.t_Choice = ~.(impl_12__is_negative s_prime <: Subtle.t_Choice) in
+  let s_prime:t_FieldElement = impl_12__conditional_negate s_prime s_prime_is_pos in
+  let s:t_FieldElement =
+    impl_12__conditional_assign s s_prime (~.v_Ns_D_is_sq <: Subtle.t_Choice)
+  in
+  let c:t_FieldElement = impl_12__conditional_assign c r (~.v_Ns_D_is_sq <: Subtle.t_Choice) in
+  let v_N_t:t_FieldElement =
+    Core_models.Ops.Arith.f_sub #t_FieldElement
+      #t_FieldElement
+      #FStar.Tactics.Typeclasses.solve
+      (Core_models.Ops.Arith.f_mul #t_FieldElement
+          #t_FieldElement
+          #FStar.Tactics.Typeclasses.solve
+          (Core_models.Ops.Arith.f_mul #t_FieldElement
+              #t_FieldElement
+              #FStar.Tactics.Typeclasses.solve
+              c
+              (Core_models.Ops.Arith.f_sub #t_FieldElement
+                  #t_FieldElement
+                  #FStar.Tactics.Typeclasses.solve
+                  r
+                  one
+                <:
+                t_FieldElement)
+            <:
+            t_FieldElement)
+          d_minus_one_sq
+        <:
+        t_FieldElement)
+      v_D
+  in
+  let s_sq:t_FieldElement = impl_12__square s in
+  RistrettoPoint
+  (impl_5__as_extended ({
+          f_X
+          =
+          Core_models.Ops.Arith.f_mul #t_FieldElement
+            #t_FieldElement
+            #FStar.Tactics.Typeclasses.solve
+            (Core_models.Ops.Arith.f_add #t_FieldElement
+                #t_FieldElement
+                #FStar.Tactics.Typeclasses.solve
+                s
+                s
+              <:
+              t_FieldElement)
+            v_D
+          <:
+          t_FieldElement;
+          f_Z
+          =
+          Core_models.Ops.Arith.f_mul #t_FieldElement
+            #t_FieldElement
+            #FStar.Tactics.Typeclasses.solve
+            v_N_t
+            v_SQRT_AD_MINUS_ONE
+          <:
+          t_FieldElement;
+          f_Y
+          =
+          Core_models.Ops.Arith.f_sub #t_FieldElement
+            #t_FieldElement
+            #FStar.Tactics.Typeclasses.solve
+            impl_12__ONE
+            s_sq
+          <:
+          t_FieldElement;
+          f_T
+          =
+          Core_models.Ops.Arith.f_add #t_FieldElement
+            #t_FieldElement
+            #FStar.Tactics.Typeclasses.solve
+            impl_12__ONE
+            s_sq
+          <:
+          t_FieldElement
+        }
+        <:
+        t_CompletedPoint))
+  <:
+  t_RistrettoPoint
+
+/// Construct a `RistrettoPoint` from 64 bytes of data.
+/// If the input bytes are uniformly distributed, the resulting
+/// point will be uniformly distributed over the group, and its
+/// discrete log with respect to other points should be unknown.
+/// # Implementation
+/// This function splits the input array into two 32-byte halves,
+/// takes the low 255 bits of each half mod p, applies the
+/// Ristretto-flavored Elligator map to each, and adds the results.
+let impl_5__from_uniform_bytes (bytes: t_Array u8 (mk_usize 64)) : t_RistrettoPoint =
+  let r_1_bytes:t_Array u8 (mk_usize 32) = Rust_primitives.Hax.repeat (mk_u8 0) (mk_usize 32) in
+  let r_1_bytes:t_Array u8 (mk_usize 32) =
+    Core_models.Slice.impl__copy_from_slice #u8
+      r_1_bytes
+      (bytes.[ {
+            Core_models.Ops.Range.f_start = mk_usize 0;
+            Core_models.Ops.Range.f_end = mk_usize 32
+          }
+          <:
+          Core_models.Ops.Range.t_Range usize ]
+        <:
+        t_Slice u8)
+  in
+  let r_1_:t_FieldElement = impl_12__from_bytes r_1_bytes in
+  let v_R_1_:t_RistrettoPoint = impl_3__elligator_ristretto_flavor r_1_ in
+  let r_2_bytes:t_Array u8 (mk_usize 32) = Rust_primitives.Hax.repeat (mk_u8 0) (mk_usize 32) in
+  let r_2_bytes:t_Array u8 (mk_usize 32) =
+    Core_models.Slice.impl__copy_from_slice #u8
+      r_2_bytes
+      (bytes.[ {
+            Core_models.Ops.Range.f_start = mk_usize 32;
+            Core_models.Ops.Range.f_end = mk_usize 64
+          }
+          <:
+          Core_models.Ops.Range.t_Range usize ]
+        <:
+        t_Slice u8)
+  in
+  let r_2_:t_FieldElement = impl_12__from_bytes r_2_bytes in
+  let v_R_2_:t_RistrettoPoint = impl_3__elligator_ristretto_flavor r_2_ in
+  Core_models.Ops.Arith.f_add #t_RistrettoPoint
+    #t_RistrettoPoint
+    #FStar.Tactics.Typeclasses.solve
+    v_R_1_
+    v_R_2_
+
 /// Attempt to compute `sqrt(1/self)` in constant time.
 /// Convenience wrapper around `sqrt_ratio_i`.
 /// This function always returns the nonnegative square root.
@@ -585,3 +1542,288 @@ let impl_12__sqrt_ratio_i (u v: t_FieldElement) : (Subtle.t_Choice & t_FieldElem
 /// - `(Choice(0), +sqrt(i/self))  ` if `self` is a nonzero nonsquare;
 let impl_12__invsqrt (self: t_FieldElement) : (Subtle.t_Choice & t_FieldElement) =
   impl_12__sqrt_ratio_i impl_12__ONE self
+
+/// Compress this point using the Ristretto encoding.
+let impl_2__compress (self: t_RistrettoPoint) : t_CompressedRistretto =
+  let v_X:t_FieldElement = self._0.f_X in
+  let v_Y:t_FieldElement = self._0.f_Y in
+  let v_Z:t_FieldElement = self._0.f_Z in
+  let v_T:t_FieldElement = self._0.f_T in
+  let u1:t_FieldElement =
+    Core_models.Ops.Arith.f_mul #t_FieldElement
+      #t_FieldElement
+      #FStar.Tactics.Typeclasses.solve
+      (Core_models.Ops.Arith.f_add #t_FieldElement
+          #t_FieldElement
+          #FStar.Tactics.Typeclasses.solve
+          v_Z
+          v_Y
+        <:
+        t_FieldElement)
+      (Core_models.Ops.Arith.f_sub #t_FieldElement
+          #t_FieldElement
+          #FStar.Tactics.Typeclasses.solve
+          v_Z
+          v_Y
+        <:
+        t_FieldElement)
+  in
+  let u2:t_FieldElement =
+    Core_models.Ops.Arith.f_mul #t_FieldElement
+      #t_FieldElement
+      #FStar.Tactics.Typeclasses.solve
+      v_X
+      v_Y
+  in
+  let (_: Subtle.t_Choice), (invsqrt: t_FieldElement) =
+    impl_12__invsqrt (Core_models.Ops.Arith.f_mul #t_FieldElement
+          #t_FieldElement
+          #FStar.Tactics.Typeclasses.solve
+          u1
+          (impl_12__square u2 <: t_FieldElement)
+        <:
+        t_FieldElement)
+  in
+  let i1:t_FieldElement =
+    Core_models.Ops.Arith.f_mul #t_FieldElement
+      #t_FieldElement
+      #FStar.Tactics.Typeclasses.solve
+      invsqrt
+      u1
+  in
+  let i2:t_FieldElement =
+    Core_models.Ops.Arith.f_mul #t_FieldElement
+      #t_FieldElement
+      #FStar.Tactics.Typeclasses.solve
+      invsqrt
+      u2
+  in
+  let z_inv:t_FieldElement =
+    Core_models.Ops.Arith.f_mul #t_FieldElement
+      #t_FieldElement
+      #FStar.Tactics.Typeclasses.solve
+      i1
+      (Core_models.Ops.Arith.f_mul #t_FieldElement
+          #t_FieldElement
+          #FStar.Tactics.Typeclasses.solve
+          i2
+          v_T
+        <:
+        t_FieldElement)
+  in
+  let den_inv:t_FieldElement = i2 in
+  let iX:t_FieldElement =
+    Core_models.Ops.Arith.f_mul #t_FieldElement
+      #t_FieldElement
+      #FStar.Tactics.Typeclasses.solve
+      v_X
+      v_SQRT_M1
+  in
+  let iY:t_FieldElement =
+    Core_models.Ops.Arith.f_mul #t_FieldElement
+      #t_FieldElement
+      #FStar.Tactics.Typeclasses.solve
+      v_Y
+      v_SQRT_M1
+  in
+  let ristretto_magic:t_FieldElement = v_INVSQRT_A_MINUS_D in
+  let enchanted_denominator:t_FieldElement =
+    Core_models.Ops.Arith.f_mul #t_FieldElement
+      #t_FieldElement
+      #FStar.Tactics.Typeclasses.solve
+      i1
+      ristretto_magic
+  in
+  let rotate:Subtle.t_Choice =
+    impl_12__is_negative (Core_models.Ops.Arith.f_mul #t_FieldElement
+          #t_FieldElement
+          #FStar.Tactics.Typeclasses.solve
+          v_T
+          z_inv
+        <:
+        t_FieldElement)
+  in
+  let v_X:t_FieldElement = impl_12__conditional_assign v_X iY rotate in
+  let v_Y:t_FieldElement = impl_12__conditional_assign v_Y iX rotate in
+  let den_inv:t_FieldElement = impl_12__conditional_assign den_inv enchanted_denominator rotate in
+  let v_Y:t_FieldElement =
+    impl_12__conditional_negate v_Y
+      (impl_12__is_negative (Core_models.Ops.Arith.f_mul #t_FieldElement
+              #t_FieldElement
+              #FStar.Tactics.Typeclasses.solve
+              v_X
+              z_inv
+            <:
+            t_FieldElement)
+        <:
+        Subtle.t_Choice)
+  in
+  let s:t_FieldElement =
+    Core_models.Ops.Arith.f_mul #t_FieldElement
+      #t_FieldElement
+      #FStar.Tactics.Typeclasses.solve
+      den_inv
+      (Core_models.Ops.Arith.f_sub #t_FieldElement
+          #t_FieldElement
+          #FStar.Tactics.Typeclasses.solve
+          v_Z
+          v_Y
+        <:
+        t_FieldElement)
+  in
+  let s_is_negative:Subtle.t_Choice = impl_12__is_negative s in
+  let s:t_FieldElement = impl_12__conditional_negate s s_is_negative in
+  CompressedRistretto (impl_12__to_bytes s) <: t_CompressedRistretto
+
+let step_2_ (s: t_FieldElement)
+    : (Subtle.t_Choice & Subtle.t_Choice & Subtle.t_Choice & t_RistrettoPoint) =
+  let one:t_FieldElement = impl_12__ONE in
+  let ss:t_FieldElement = impl_12__square s in
+  let u1:t_FieldElement =
+    Core_models.Ops.Arith.f_sub #t_FieldElement
+      #t_FieldElement
+      #FStar.Tactics.Typeclasses.solve
+      one
+      ss
+  in
+  let u2:t_FieldElement =
+    Core_models.Ops.Arith.f_add #t_FieldElement
+      #t_FieldElement
+      #FStar.Tactics.Typeclasses.solve
+      one
+      ss
+  in
+  let u2_sqr:t_FieldElement = impl_12__square u2 in
+  let v:t_FieldElement =
+    Core_models.Ops.Arith.f_sub #t_FieldElement
+      #t_FieldElement
+      #FStar.Tactics.Typeclasses.solve
+      (Core_models.Ops.Arith.f_mul #t_FieldElement
+          #t_FieldElement
+          #FStar.Tactics.Typeclasses.solve
+          (Core_models.Ops.Arith.f_neg #t_FieldElement #FStar.Tactics.Typeclasses.solve v_EDWARDS_D
+            <:
+            t_FieldElement)
+          (impl_12__square u1 <: t_FieldElement)
+        <:
+        t_FieldElement)
+      u2_sqr
+  in
+  let (ok: Subtle.t_Choice), (v_I: t_FieldElement) =
+    impl_12__invsqrt (Core_models.Ops.Arith.f_mul #t_FieldElement
+          #t_FieldElement
+          #FStar.Tactics.Typeclasses.solve
+          v
+          u2_sqr
+        <:
+        t_FieldElement)
+  in
+  let v_Dx:t_FieldElement =
+    Core_models.Ops.Arith.f_mul #t_FieldElement
+      #t_FieldElement
+      #FStar.Tactics.Typeclasses.solve
+      v_I
+      u2
+  in
+  let v_Dy:t_FieldElement =
+    Core_models.Ops.Arith.f_mul #t_FieldElement
+      #t_FieldElement
+      #FStar.Tactics.Typeclasses.solve
+      v_I
+      (Core_models.Ops.Arith.f_mul #t_FieldElement
+          #t_FieldElement
+          #FStar.Tactics.Typeclasses.solve
+          v_Dx
+          v
+        <:
+        t_FieldElement)
+  in
+  let x:t_FieldElement =
+    Core_models.Ops.Arith.f_mul #t_FieldElement
+      #t_FieldElement
+      #FStar.Tactics.Typeclasses.solve
+      (Core_models.Ops.Arith.f_add #t_FieldElement
+          #t_FieldElement
+          #FStar.Tactics.Typeclasses.solve
+          s
+          s
+        <:
+        t_FieldElement)
+      v_Dx
+  in
+  let x_neg:Subtle.t_Choice = impl_12__is_negative x in
+  let x:t_FieldElement = impl_12__conditional_negate x x_neg in
+  let y:t_FieldElement =
+    Core_models.Ops.Arith.f_mul #t_FieldElement
+      #t_FieldElement
+      #FStar.Tactics.Typeclasses.solve
+      u1
+      v_Dy
+  in
+  let t:t_FieldElement =
+    Core_models.Ops.Arith.f_mul #t_FieldElement #t_FieldElement #FStar.Tactics.Typeclasses.solve x y
+  in
+  ok,
+  impl_12__is_negative t,
+  impl_12__is_zero y,
+  (RistrettoPoint ({ f_X = x; f_Y = y; f_Z = one; f_T = t } <: t_EdwardsPoint) <: t_RistrettoPoint)
+  <:
+  (Subtle.t_Choice & Subtle.t_Choice & Subtle.t_Choice & t_RistrettoPoint)
+
+/// Attempt to decompress to an `RistrettoPoint`.
+/// # Return
+/// - `Some(RistrettoPoint)` if `self` was the canonical encoding of a point;
+/// - `None` if `self` was not the canonical encoding of a point.
+let impl_19__decompress (self: t_CompressedRistretto) : Core_models.Option.t_Option t_RistrettoPoint =
+  let
+  (s_encoding_is_canonical: Subtle.t_Choice), (s_is_negative: Subtle.t_Choice), (s: t_FieldElement)
+  =
+    step_1_ self
+  in
+  if
+    Core_models.Convert.f_into #Subtle.t_Choice
+      #bool
+      #FStar.Tactics.Typeclasses.solve
+      (Core_models.Ops.Bit.f_bitor #Subtle.t_Choice
+          #Subtle.t_Choice
+          #FStar.Tactics.Typeclasses.solve
+          (~.s_encoding_is_canonical <: Subtle.t_Choice)
+          s_is_negative
+        <:
+        Subtle.t_Choice)
+  then Core_models.Option.Option_None <: Core_models.Option.t_Option t_RistrettoPoint
+  else
+    let
+    (ok: Subtle.t_Choice),
+    (tt_is_negative: Subtle.t_Choice),
+    (y_is_zero: Subtle.t_Choice),
+    (res: t_RistrettoPoint) =
+      step_2_ s
+    in
+    if
+      Core_models.Convert.f_into #Subtle.t_Choice
+        #bool
+        #FStar.Tactics.Typeclasses.solve
+        (Core_models.Ops.Bit.f_bitor #Subtle.t_Choice
+            #Subtle.t_Choice
+            #FStar.Tactics.Typeclasses.solve
+            (Core_models.Ops.Bit.f_bitor #Subtle.t_Choice
+                #Subtle.t_Choice
+                #FStar.Tactics.Typeclasses.solve
+                (~.ok <: Subtle.t_Choice)
+                tt_is_negative
+              <:
+              Subtle.t_Choice)
+            y_is_zero
+          <:
+          Subtle.t_Choice)
+    then Core_models.Option.Option_None <: Core_models.Option.t_Option t_RistrettoPoint
+    else Core_models.Option.Option_Some res <: Core_models.Option.t_Option t_RistrettoPoint
+
+/// Return the Ristretto255 basepoint.
+let impl_5__basepoint (_: Prims.unit) : t_RistrettoPoint =
+  Core_models.Option.impl__expect #t_RistrettoPoint
+    (impl_19__decompress v_RISTRETTO_BASEPOINT_COMPRESSED
+      <:
+      Core_models.Option.t_Option t_RistrettoPoint)
+    "hardcoded basepoint is valid"
