ristretto255/proofs/fstar/extraction/Ristretto255.Backend.fst
@@ -1,0 +1,38 @@
+module Ristretto255.Backend
+#set-options "--fuel 0 --ifuel 1 --z3rlimit 15"
+open FStar.Mul
+open Core_models
+
+include Ristretto255.Bundle {t_EdwardsPoint as t_EdwardsPoint}
+
+include Ristretto255.Bundle {impl_7__from__backend as impl_7}
+
+include Ristretto255.Bundle {impl_8__from__backend as impl_8}
+
+include Ristretto255.Bundle {impl__from__backend as impl}
+
+include Ristretto255.Bundle {impl_1__from__backend as impl_1}
+
+include Ristretto255.Bundle {impl_2 as impl_2}
+
+include Ristretto255.Bundle {impl_3 as impl_3}
+
+include Ristretto255.Bundle {impl_4__as_projective_niels as impl_EdwardsPoint__as_projective_niels}
+
+include Ristretto255.Bundle {impl_4__as_extended as impl_EdwardsPoint__as_extended}
+
+include Ristretto255.Bundle {t_CompletedPoint as t_CompletedPoint}
+
+include Ristretto255.Bundle {impl_9__from__backend as impl_9}
+
+include Ristretto255.Bundle {impl_10__from__backend as impl_10}
+
+include Ristretto255.Bundle {impl_5__as_extended as impl_CompletedPoint__as_extended}
+
+include Ristretto255.Bundle {t_ProjectiveNielsPoint as t_ProjectiveNielsPoint}
+
+include Ristretto255.Bundle {impl_11__from__backend as impl_11}
+
+include Ristretto255.Bundle {impl_12__from__backend as impl_12}
+
+include Ristretto255.Bundle {impl_6__from__backend as impl_6}
