ristretto255/proofs/fstar/extraction/Ristretto255.Scalar.fst
@@ -1,0 +1,83 @@
+module Ristretto255.Scalar
+#set-options "--fuel 0 --ifuel 1 --z3rlimit 15"
+open FStar.Mul
+open Core_models
+
+let _ =
+  (* This module has implicit dependencies, here we make them explicit. *)
+  (* The implicit dependencies arise from typeclasses instances. *)
+  let open Rand_core in
+  ()
+
+/// A scalar value for the ristretto255 group.
+/// Scalars are integers mod ℓ, where ℓ is the order of the ristretto255 group.
+type t_Scalar = | Scalar : t_Array u8 (mk_usize 32) -> t_Scalar
+
+let impl_1: Core_models.Clone.t_Clone t_Scalar =
+  { f_clone = (fun x -> x); f_clone_pre = (fun _ -> True); f_clone_post = (fun _ _ -> True) }
+
+[@@ FStar.Tactics.Typeclasses.tcinstance]
+assume
+val impl_2': Core_models.Fmt.t_Debug t_Scalar
+
+unfold
+let impl_2 = impl_2'
+
+[@@ FStar.Tactics.Typeclasses.tcinstance]
+assume
+val impl_3': Core_models.Marker.t_StructuralPartialEq t_Scalar
+
+unfold
+let impl_3 = impl_3'
+
+[@@ FStar.Tactics.Typeclasses.tcinstance]
+assume
+val impl_4': Core_models.Cmp.t_PartialEq t_Scalar t_Scalar
+
+unfold
+let impl_4 = impl_4'
+
+[@@ FStar.Tactics.Typeclasses.tcinstance]
+assume
+val impl_5': Core_models.Cmp.t_Eq t_Scalar
+
+unfold
+let impl_5 = impl_5'
+
+/// Generate a random scalar using the provided RNG.
+assume
+val impl_Scalar__random':
+    #v_R: Type0 ->
+    {| i0: Rand_core.t_RngCore v_R |} ->
+    {| i1: Rand_core.t_CryptoRng v_R |} ->
+    e_rng: v_R
+  -> (v_R & t_Scalar)
+
+unfold
+let impl_Scalar__random
+      (#v_R: Type0)
+      (#[FStar.Tactics.Typeclasses.tcresolve ()] i0: Rand_core.t_RngCore v_R)
+      (#[FStar.Tactics.Typeclasses.tcresolve ()] i1: Rand_core.t_CryptoRng v_R)
+     = impl_Scalar__random' #v_R #i0 #i1
+
+/// Attempt to construct a scalar from a canonical byte representation.
+/// Returns `None` if the bytes do not represent a canonical scalar
+/// (i.e. the value is >= ℓ).
+assume
+val impl_Scalar__from_bytes_checked': e_bytes: t_Array u8 (mk_usize 32)
+  -> Core_models.Option.t_Option t_Scalar
+
+unfold
+let impl_Scalar__from_bytes_checked = impl_Scalar__from_bytes_checked'
+
+/// Construct a scalar by reducing a 256-bit little-endian integer modulo ℓ.
+/// Unlike [`from_bytes_checked`](Self::from_bytes_checked), this always
+/// succeeds by reducing the input mod the group order.
+assume
+val impl_Scalar__from_bytes_mod_order': e_bytes: t_Array u8 (mk_usize 32) -> t_Scalar
+
+unfold
+let impl_Scalar__from_bytes_mod_order = impl_Scalar__from_bytes_mod_order'
+
+/// Serialize this scalar to a 32-byte little-endian array.
+let impl_Scalar__to_bytes (self: t_Scalar) : t_Array u8 (mk_usize 32) = self._0
