ristretto255/proofs/fstar/extraction/Ristretto255.fst
@@ -3,38 +3,66 @@ module Ristretto255
 open FStar.Mul
 open Core_models
 
-include Ristretto255.Bundle_decompress {t_CompressedRistretto as t_CompressedRistretto}
+include Ristretto255.Bundle {t_CompressedRistretto as t_CompressedRistretto}
 
-include Ristretto255.Bundle_decompress {CompressedRistretto as CompressedRistretto}
+include Ristretto255.Bundle {CompressedRistretto as CompressedRistretto}
 
-include Ristretto255.Bundle_decompress {impl_2 as impl_2}
+include Ristretto255.Bundle {impl_12 as impl_12}
 
-include Ristretto255.Bundle_decompress {impl_3 as impl_3}
+include Ristretto255.Bundle {impl_13 as impl_13}
 
-include Ristretto255.Bundle_decompress {impl_4 as impl_4}
+include Ristretto255.Bundle {impl_14 as impl_14}
 
-include Ristretto255.Bundle_decompress {impl_5 as impl_5}
+include Ristretto255.Bundle {impl_15 as impl_15}
 
-include Ristretto255.Bundle_decompress {impl_6 as impl_6}
+include Ristretto255.Bundle {impl_16 as impl_16}
 
-include Ristretto255.Bundle_decompress {impl_7 as impl_7}
+include Ristretto255.Bundle {impl_17 as impl_17}
 
-include Ristretto255.Bundle_decompress {impl_8__to_bytes as impl_CompressedRistretto__to_bytes}
+include Ristretto255.Bundle {impl_18 as impl_18}
 
-include Ristretto255.Bundle_decompress {impl_8__as_bytes as impl_CompressedRistretto__as_bytes}
+include Ristretto255.Bundle {impl_19__to_bytes as impl_CompressedRistretto__to_bytes}
 
-include Ristretto255.Bundle_decompress {impl_8__from_slice as impl_CompressedRistretto__from_slice}
+include Ristretto255.Bundle {impl_19__as_bytes as impl_CompressedRistretto__as_bytes}
 
-include Ristretto255.Bundle_decompress {impl_8__decompress as impl_CompressedRistretto__decompress}
+include Ristretto255.Bundle {impl_19__from_slice as impl_CompressedRistretto__from_slice}
 
-include Ristretto255.Bundle_decompress {impl as impl}
+include Ristretto255.Bundle {impl_19__decompress as impl_CompressedRistretto__decompress}
 
-include Ristretto255.Bundle_decompress {impl_1 as impl_1}
+include Ristretto255.Bundle {impl as impl}
 
-include Ristretto255.Bundle_decompress {impl_9 as impl_9}
+include Ristretto255.Bundle {impl_1 as impl_1}
 
-include Ristretto255.Bundle_decompress {t_RistrettoPoint as t_RistrettoPoint}
+include Ristretto255.Bundle {impl_20 as impl_20}
 
-include Ristretto255.Bundle_decompress {RistrettoPoint as RistrettoPoint}
+include Ristretto255.Bundle {t_RistrettoPoint as t_RistrettoPoint}
 
-include Ristretto255.Bundle_decompress {t_EdwardsPoint as t_EdwardsPoint}
+include Ristretto255.Bundle {RistrettoPoint as RistrettoPoint}
+
+include Ristretto255.Bundle {impl_21 as impl_21}
+
+include Ristretto255.Bundle {impl_22 as impl_22}
+
+include Ristretto255.Bundle {impl_23 as impl_23}
+
+include Ristretto255.Bundle {impl_2__compress as impl_RistrettoPoint__compress}
+
+include Ristretto255.Bundle {impl_3__elligator_ristretto_flavor as impl_RistrettoPoint__elligator_ristretto_flavor}
+
+include Ristretto255.Bundle {impl_4 as impl_4}
+
+include Ristretto255.Bundle {impl_5__basepoint as impl_RistrettoPoint__basepoint}
+
+include Ristretto255.Bundle {impl_5__from_uniform_bytes as impl_RistrettoPoint__from_uniform_bytes}
+
+include Ristretto255.Bundle {impl_6 as impl_6}
+
+include Ristretto255.Bundle {impl_7 as impl_7}
+
+include Ristretto255.Bundle {impl_8 as impl_8}
+
+include Ristretto255.Bundle {impl_9 as impl_9}
+
+include Ristretto255.Bundle {impl_10 as impl_10}
+
+include Ristretto255.Bundle {impl_11 as impl_11}
