ristretto255/proofs/fstar/extraction/Ristretto255.Constants.fst
@@ -6,3 +6,17 @@ open Core_models
 include Ristretto255.Bundle {v_EDWARDS_D as v_EDWARDS_D}
 
 include Ristretto255.Bundle {v_SQRT_M1 as v_SQRT_M1}
+
+include Ristretto255.Bundle {v_INVSQRT_A_MINUS_D as v_INVSQRT_A_MINUS_D}
+
+include Ristretto255.Bundle {v_ONE_MINUS_EDWARDS_D_SQUARED as v_ONE_MINUS_EDWARDS_D_SQUARED}
+
+include Ristretto255.Bundle {v_EDWARDS_D_MINUS_ONE_SQUARED as v_EDWARDS_D_MINUS_ONE_SQUARED}
+
+include Ristretto255.Bundle {v_SQRT_AD_MINUS_ONE as v_SQRT_AD_MINUS_ONE}
+
+include Ristretto255.Bundle {v_MINUS_ONE as v_MINUS_ONE}
+
+include Ristretto255.Bundle {v_EDWARDS_D2 as v_EDWARDS_D2}
+
+include Ristretto255.Bundle {v_RISTRETTO_BASEPOINT_COMPRESSED as v_RISTRETTO_BASEPOINT_COMPRESSED}
